vale/code/arch/x64/interop/new/Vale.AsLowStar.MemoryHelpers.fst
@@ -1,0 +1,57 @@
+module Vale.AsLowStar.MemoryHelpers
+
+open Interop.Base
+module B = LowStar.Buffer
+module BS = X64.Bytes_Semantics_s
+module BV = LowStar.BufferView
+module HS = FStar.HyperStack
+module ME = X64.Memory
+module MES = X64.Memory_Sems
+module TS = X64.Taint_Semantics_s
+module MS = X64.Machine_s
+module IA = Interop.Assumptions
+module IM = Interop.Mem
+module V = X64.Vale.Decls
+module VS = X64.Vale.State
+module IX64 = Interop.X64
+module VSig = Vale.AsLowStar.ValeSig
+module LSig = Vale.AsLowStar.LowStarSig
+module SL = X64.Vale.StateLemmas
+module VL = X64.Vale.Lemmas
+module ST = FStar.HyperStack.ST
+
+friend X64.Memory
+friend X64.Memory_Sems
+
+open Interop.Adapters
+
+let down_mem_unify () : Lemma (IM.down_mem == Interop.down_mem) = 
+  admit() // TODO: We should only have one def for down_mem
+
+let mk_mem_reveal (args:list arg) (h0:mem_roots args) : Lemma
+  (let mem = mk_mem args h0 in
+   hs_of_mem mem == mem.ME.hs /\
+   ptrs_of_mem mem == mem.ME.ptrs /\
+   IA.addrs == mem.ME.addrs) =
+   admit() // TODO: Will be provable with an implementation for Interop.Adapters
+
+let buffer_readable_reveal bt x args h0 stack =
+  let mem = mk_mem (arg_of_lb stack::args) h0 in
+  mk_mem_injective (arg_of_lb stack::args) h0;
+  mk_mem_reveal (arg_of_lb stack::args) h0
+
+let get_heap_mk_mem_reveal args h0 stack =
+  let mem = mk_mem (arg_of_lb stack::args) h0 in
+  mk_mem_injective (arg_of_lb stack::args) h0;
+  down_mem_unify ();
+  mk_mem_reveal (arg_of_lb stack::args) h0
+
+let buffer_as_seq_reveal t x args h0 stack =
+  let y = as_vale_buffer x in
+  let mem = mk_mem (arg_of_lb stack::args) h0 in
+  assume (t <> ME.TUInt128); // TODO: TUInt128
+  mk_mem_injective (arg_of_lb stack::args) h0;
+  mk_mem_reveal (arg_of_lb stack::args) h0
+
+let buffer_addr_reveal t x args h0 =
+  mk_mem_reveal args h0
